Refactored let-floating a bit

00Utils/Utils.thy
@@ -11,53 +11,47 @@ subsection \<open>Utilities\<close>
 text \<open>In this section we have a number of miscellaneous functions and lemmas about the standard 
 library that do not fit anywhere else. This can be skimmed or skipped on a first read.\<close>
 
-primrec map_with_idx :: "(nat \<Rightarrow> 'a \<Rightarrow> 'b) \<Rightarrow> 'a list \<Rightarrow> 'b list" where
-  "map_with_idx f [] = []"
-| "map_with_idx f (a # as) = f 0 a # map_with_idx (f \<circ> Suc) as"
+primrec map_with_idx :: "nat \<Rightarrow> (nat \<Rightarrow> 'a \<Rightarrow> 'b) \<Rightarrow> 'a list \<Rightarrow> 'b list" where
+  "map_with_idx x f [] = []"
+| "map_with_idx x f (a # as) = f x a # map_with_idx (Suc x) f as"
 
-lemma map_with_idx_id [simp]: "map_with_idx (\<lambda>a b. b) as = as"
-  by (induction as) (simp_all add: comp_def)
+lemma map_with_idx_id [simp]: "map_with_idx x (\<lambda>a b. b) as = as"
+  by (induction as arbitrary: x) (simp_all add: comp_def)
 
-lemma map_with_idx_const [simp]: "map_with_idx (\<lambda>k. f) as = map f as"
-  by (induction as) (simp_all add: comp_def)
+lemma map_with_idx_const [simp]: "map_with_idx x (\<lambda>k. f) as = map f as"
+  by (induction as arbitrary: x) (simp_all add: comp_def)
 
-lemma length_map_with_idx [simp]: "length (map_with_idx f as) = length as"
-  by (induction as arbitrary: f) simp_all
+lemma length_map_with_idx [simp]: "length (map_with_idx x f as) = length as"
+  by (induction as arbitrary: x) simp_all
 
-lemma map_with_idx_append [simp]: "map_with_idx f (as @ bs) = 
-    map_with_idx f as @ map_with_idx (f \<circ> (+) (length as)) bs"
-  by (induction as arbitrary: f) (simp_all add: comp_def)
+lemma map_with_idx_append [simp]: "map_with_idx x f (as @ bs) = 
+    map_with_idx x f as @ map_with_idx (x + length as) f bs"
+  by (induction as arbitrary: x) (simp_all add: comp_def)
 
-lemma len_conc_map_ix_lemma' [simp]: "((\<lambda>x. f (ix + x)) \<circ> Suc) = (\<lambda>x. f (Suc (ix + x)))"
+lemma length_concat_map_with_idx [simp]: "length (concat (map_with_idx x f as)) = 
+    sum_list (map_with_idx x (\<lambda>ix a. length (f ix a)) as)"
+  by (induction as arbitrary: x) simp_all
+
+lemma map_with_idx_comp' [simp]: "map_with_idx x (\<lambda>k. f k \<circ> g k) as = 
+    map_with_idx x f (map_with_idx x g as)"
+  by (induction as arbitrary: x) (simp_all add: comp_def)
+
+lemma map_with_idx_comp [simp]: "map_with_idx x (\<lambda>k. f k \<circ> g k) = 
+    map_with_idx x f \<circ> map_with_idx x g"
   by auto
 
-lemma len_conc_map_ix_lemma [simp]: "((\<lambda>ix a. length (f ix a)) \<circ> Suc) = 
-    (\<lambda>ix a. length (f (Suc ix) a))"
+lemma map_with_idx_comp2' [simp]: "map_with_idx x (\<lambda>k. f \<circ> g k) as = map f (map_with_idx x g as)"
+  by (induction as arbitrary: x) (simp_all add: comp_def)
+
+lemma map_with_idx_comp2 [simp]: "map_with_idx x (\<lambda>k. f \<circ> g k) = map f \<circ> map_with_idx x g"
   by auto
 
-lemma length_concat_map_with_idx [simp]: "length (concat (map_with_idx f as)) = 
-    sum_list (map_with_idx (\<lambda>ix a. length (f ix a)) as)"
-  by (induction as arbitrary: f) simp_all
-
-lemma map_with_idx_comp' [simp]: "map_with_idx (\<lambda>k. f k \<circ> g k) as = 
-    map_with_idx f (map_with_idx g as)"
-  by (induction as arbitrary: f g) (simp_all add: comp_def)
-
-lemma map_with_idx_comp [simp]: "map_with_idx (\<lambda>k. f k \<circ> g k) = map_with_idx f \<circ> map_with_idx g"
-  by auto
-
-lemma map_with_idx_lemma [simp]: "(\<lambda>k. f \<circ> g k) \<circ> Suc = (\<lambda>k. f \<circ> g (Suc k))"
-  by auto
-
-lemma map_with_idx_comp2' [simp]: "map_with_idx (\<lambda>k. f \<circ> g k) as = map f (map_with_idx g as)"
-  by (induction as arbitrary: g) (simp_all add: comp_def)
-
-lemma map_with_idx_comp2 [simp]: "map_with_idx (\<lambda>k. f \<circ> g k) = map f \<circ> map_with_idx g"
-  by auto
+lemma map_with_idx_suc [simp]: "map_with_idx x (f \<circ> Suc) as = map_with_idx (Suc x) f as"
+  by (induction as arbitrary: x) simp_all
 
 lemma list_all_map_with_idx [simp]: "(\<And>k a. p (f k a) = p a) \<Longrightarrow> 
-    list_all p (map_with_idx f as) = list_all p as"
-  by (induction as arbitrary: f) simp_all
+    list_all p (map_with_idx x f as) = list_all p as"
+  by (induction as arbitrary: x) simp_all
 
 fun nat_to_string' :: "nat \<Rightarrow> char" where
   "nat_to_string' 0 = CHR 48"
