03Debruijn/LetFloating.thy
@@ -45,6 +45,11 @@ the "Further Work" section at the end.\<close>
 
 text \<open>We begin by defining our let-floated normal form.\<close>
 
+fun is_reducible :: "expr\<^sub>d \<Rightarrow> bool" where
+  "is_reducible (App\<^sub>d e\<^sub>1 e\<^sub>2) = True"
+| "is_reducible (Let\<^sub>d e\<^sub>1 e\<^sub>2) = True"
+| "is_reducible e = False"
+
 primrec let_free :: "expr\<^sub>d \<Rightarrow> bool" where
   "let_free (Var\<^sub>d x) = True"
 | "let_free (Const\<^sub>d n) = True"
@@ -56,8 +61,18 @@ primrec let_floated :: "expr\<^sub>d \<Rightarrow> bool" where
   "let_floated (Var\<^sub>d x) = True"
 | "let_floated (Const\<^sub>d n) = True"
 | "let_floated (Lam\<^sub>d t e) = let_floated e"
-| "let_floated (App\<^sub>d e\<^sub>1 e\<^sub>2) = (let_free e\<^sub>1 \<and> let_free e\<^sub>2 \<and> let_floated e\<^sub>1 \<and> let_floated e\<^sub>2)"
+| "let_floated (App\<^sub>d e\<^sub>1 e\<^sub>2) = 
+    (let_free e\<^sub>1 \<and> let_free e\<^sub>2 \<and> \<not> is_reducible e\<^sub>1 \<and> let_floated e\<^sub>1 \<and> let_floated e\<^sub>2)"
 | "let_floated (Let\<^sub>d e\<^sub>1 e\<^sub>2) = (let_free e\<^sub>1 \<and> let_floated e\<^sub>1 \<and> let_floated e\<^sub>2)"
+
+lemma value_not_reducible [simp]: "value\<^sub>d v \<Longrightarrow> \<not> is_reducible v"
+  by (induction v) simp_all
+
+lemma is_reducible_incr [simp]: "is_reducible (incr\<^sub>d x e) = is_reducible e"
+  by (induction e) simp_all
+
+lemma is_reducible_subst [simp]: "value\<^sub>d v \<Longrightarrow> is_reducible (subst\<^sub>d x v e) = is_reducible e"
+  by (induction e) simp_all
 
 text \<open>Then, the let-floating transformation itself. We have to define a multiple-increment function
 to make sure the variables match properly.\<close>
@@ -66,14 +81,7 @@ primrec multiincr :: "nat \<Rightarrow> nat \<Rightarrow> expr\<^sub>d \<Rightar
   "multiincr 0 y = id"
 | "multiincr (Suc x) y = incr\<^sub>d y \<circ> multiincr x y"
 
-lemma multiincr_var [simp]: "multiincr x 0 (Var\<^sub>d 0) = Var\<^sub>d x"
-  by (induction x) simp_all
-
 lemma multiincr_incr_swap' [simp]: "multiincr x y (incr\<^sub>d y e) = incr\<^sub>d y (multiincr x y e)"
-  by (induction x) simp_all
-
-lemma multiincr_subst_swap' [simp]: "y \<le> z \<Longrightarrow> 
-    multiincr x y (subst\<^sub>d z e' e) = subst\<^sub>d (x + z) (multiincr x y e') (multiincr x y e)"
   by (induction x) simp_all
 
 lemma multiincr_incr_swap [simp]: "z \<ge> y \<Longrightarrow> 
@@ -97,6 +105,9 @@ lemma multiincr_val [simp]: "value\<^sub>d (multiincr x y e) = value\<^sub>d e"
 lemma incr_multiincr_higher: "incr\<^sub>d y (multiincr x y e) = incr\<^sub>d (x + y) (multiincr x y e)"
   by (induction x) simp_all
 
+lemma multiincr_var [simp]: "multiincr x y (Var\<^sub>d z) = Var\<^sub>d (if z < y then z else z + x)"
+  by (induction x) (simp_all add: incr_above incr_le)
+
 lemma multiincr_lam [simp]: "multiincr x y (Lam\<^sub>d t e) = Lam\<^sub>d t (multiincr x (Suc y) e)"
   by (induction x) simp_all
 
@@ -107,12 +118,19 @@ lemma multiincr_let [simp]: "multiincr x y (Let\<^sub>d e\<^sub>1 e\<^sub>2) =
     Let\<^sub>d (multiincr x y e\<^sub>1) (multiincr x (Suc y) e\<^sub>2)"
   by (induction x) simp_all
 
+lemma multiincr_subst_swap' [simp]: "y \<le> z \<Longrightarrow> 
+    multiincr x y (subst\<^sub>d z e' e) = subst\<^sub>d (x + z) (multiincr x y e') (multiincr x y e)"
+  by (induction x) simp_all
+
 lemma multiincr_subst [simp]: "z \<le> y \<Longrightarrow> multiincr x y (subst\<^sub>d z e' e) = 
     subst\<^sub>d z (multiincr x y e') (multiincr x (Suc y) e)"
   by (induction x) simp_all
 
 lemma eval_multiincr [simp]: "e \<leadsto>\<^sub>d e' \<Longrightarrow> multiincr x y e \<leadsto>\<^sub>d multiincr x y e'"
   by (induction e e' rule: eval\<^sub>d.induct) simp_all
+
+lemma is_reducible_multiincr [simp]: "is_reducible (multiincr x y e) = is_reducible e"
+  by (induction e) simp_all
 
 fun strip_lets :: "expr\<^sub>d \<Rightarrow> expr\<^sub>d list" where
   "strip_lets (Let\<^sub>d e\<^sub>1 e\<^sub>2) = e\<^sub>1 # strip_lets e\<^sub>2"
@@ -143,17 +161,7 @@ lemma reapply_nil [simp]: "reapply_lets [] e = e"
 lemma reapply_append [simp]: "reapply_lets (es @ es') e = reapply_lets es (reapply_lets es' e)"
   by (simp add: reapply_lets_def)
 
-fun is_reducible :: "expr\<^sub>d \<Rightarrow> bool" where
-  "is_reducible (App\<^sub>d e\<^sub>1 e\<^sub>2) = True"
-| "is_reducible e = False"
-
-lemma value_not_reducible [simp]: "value\<^sub>d v \<Longrightarrow> \<not> is_reducible v"
-  by (induction v) simp_all
-
-lemma is_reducible_incr [simp]: "is_reducible (incr\<^sub>d x e) = is_reducible e"
-  by (induction e) simp_all
-
-lemma is_reducible_subst [simp]: "value\<^sub>d v \<Longrightarrow> is_reducible (subst\<^sub>d x v e) = is_reducible e"
+lemma inner_expr_reducible [simp]: "\<not> is_reducible e \<Longrightarrow> \<not> is_reducible (inner_expr e)"
   by (induction e) simp_all
 
 primrec float_lets :: "expr\<^sub>d \<Rightarrow> expr\<^sub>d" where
@@ -167,7 +175,7 @@ primrec float_lets :: "expr\<^sub>d \<Rightarrow> expr\<^sub>d" where
     in let e\<^sub>2' = inner_expr (float_lets e\<^sub>2) 
     in let es\<^sub>1' = if is_reducible e\<^sub>1' then es\<^sub>1 @ [e\<^sub>1'] else es\<^sub>1
     in let e\<^sub>1'' = if is_reducible e\<^sub>1' then Var\<^sub>d 0 else e\<^sub>1'
-    in reapply_lets (es\<^sub>1' @ map_with_idx (multiincr (length es\<^sub>1')) es\<^sub>2) 
+    in reapply_lets (es\<^sub>1' @ map_with_idx 0 (multiincr (length es\<^sub>1')) es\<^sub>2) 
          (App\<^sub>d (multiincr (length es\<^sub>2) 0 e\<^sub>1'') (multiincr (length es\<^sub>1') (length es\<^sub>2) e\<^sub>2')))"
 | "float_lets (Let\<^sub>d e\<^sub>1 e\<^sub>2) = (
     let es\<^sub>1 = strip_lets (float_lets e\<^sub>1)
@@ -212,6 +220,18 @@ lemma reapply_lets_normalized [simp]: "let_floated (reapply_lets es e) =
 lemma float_lets_normalizes [simp]: "let_floated (float_lets e)"
   by (induction e) (simp_all add: Let_def)
 
+lemma let_free_strip_lets [simp]: "let_free e \<Longrightarrow> strip_lets e = []"
+  by (induction e) simp_all
+
+lemma let_free_inner_expr [simp]: "let_free e \<Longrightarrow> inner_expr e = e"
+  by (induction e) simp_all
+
+lemma float_lets_let_floated [simp]: "let_floated e \<Longrightarrow> float_lets e = e"
+  by (induction e) simp_all
+
+lemma float_lets_idempotent [simp]: "float_lets (float_lets e) = float_lets e"
+  by simp
+
 text \<open>And the safety and correctness proofs:\<close>
 
 inductive typing\<^sub>d_bindings :: "ty list \<Rightarrow> expr\<^sub>d list \<Rightarrow> ty list \<Rightarrow> bool" (infix "\<turnstile>\<^sub>d\<^sub>b _ :" 50) where
@@ -234,8 +254,9 @@ qed auto
 lemma typing_bindings_eq_length [simp]: "\<Gamma> \<turnstile>\<^sub>d\<^sub>b es : ts \<Longrightarrow> length es = length ts"
   by (induction \<Gamma> es ts rule: typing\<^sub>d_bindings.induct) simp_all
 
-lemma typing_bindings_eq_length_map [simp]: "\<Gamma> \<turnstile>\<^sub>d\<^sub>b map_with_idx f es : ts \<Longrightarrow> length es = length ts"
-proof (induction es arbitrary: \<Gamma> f ts)
+lemma typing_bindings_eq_length_map [simp]: "\<Gamma> \<turnstile>\<^sub>d\<^sub>b map_with_idx x f es : ts \<Longrightarrow> 
+  length es = length ts"
+proof (induction es arbitrary: \<Gamma> x ts)
   case (Cons e es)
   thus ?case by (induction ts rule: rev_induct) auto
 qed auto
@@ -251,40 +272,40 @@ proof (induction \<Gamma>')
 qed simp_all
 
 lemma typing_binding_incr [simp]: "\<Gamma>\<^sub>1 @ \<Gamma>\<^sub>2 \<turnstile>\<^sub>d\<^sub>b es : ts \<Longrightarrow> 
-  \<Gamma>\<^sub>1 @ t # \<Gamma>\<^sub>2 \<turnstile>\<^sub>d\<^sub>b map_with_idx (\<lambda>k. incr\<^sub>d (k + length \<Gamma>\<^sub>1)) es : ts" 
+  \<Gamma>\<^sub>1 @ t # \<Gamma>\<^sub>2 \<turnstile>\<^sub>d\<^sub>b map_with_idx (length \<Gamma>\<^sub>1) incr\<^sub>d es : ts" 
 proof (induction es arbitrary: \<Gamma>\<^sub>1 ts)
   case (Cons e es)
   then obtain ts' t' where T: "(\<Gamma>\<^sub>1 @ \<Gamma>\<^sub>2 \<turnstile>\<^sub>d e : t') \<and> (insert_at 0 t' (\<Gamma>\<^sub>1 @ \<Gamma>\<^sub>2) \<turnstile>\<^sub>d\<^sub>b es : ts') \<and> 
     ts = ts' @ [t']" by fastforce
   hence "insert_at 0 t' \<Gamma>\<^sub>1 @ \<Gamma>\<^sub>2 \<turnstile>\<^sub>d\<^sub>b es : ts'" by simp
   with Cons have "insert_at 0 t' \<Gamma>\<^sub>1 @ t # \<Gamma>\<^sub>2 \<turnstile>\<^sub>d\<^sub>b 
-    map_with_idx (\<lambda>k. incr\<^sub>d (k + length (insert_at 0 t' \<Gamma>\<^sub>1))) es : ts'" by blast
-  hence X: "insert_at 0 t' (\<Gamma>\<^sub>1 @ t # \<Gamma>\<^sub>2) \<turnstile>\<^sub>d\<^sub>b 
-    map_with_idx ((\<lambda>k. incr\<^sub>d (k + length \<Gamma>\<^sub>1)) \<circ> Suc) es : ts'" by (simp add: comp_def)
+    map_with_idx (length (insert_at 0 t' \<Gamma>\<^sub>1)) incr\<^sub>d es : ts'" by blast
+  hence X: "insert_at 0 t' (\<Gamma>\<^sub>1 @ t # \<Gamma>\<^sub>2) \<turnstile>\<^sub>d\<^sub>b map_with_idx (Suc (length \<Gamma>\<^sub>1)) incr\<^sub>d es : ts'" 
+    by (simp add: comp_def)
   from T have "insert_at (length \<Gamma>\<^sub>1) t (\<Gamma>\<^sub>1 @ \<Gamma>\<^sub>2) \<turnstile>\<^sub>d incr\<^sub>d (length \<Gamma>\<^sub>1) e : t'"
     by (metis tc\<^sub>d_incr le_add1 length_append)
   with T X show ?case by simp
 qed auto
 
 lemma typing_binding_multiincr' [simp]: "\<Gamma>\<^sub>1 @ \<Gamma>\<^sub>2 \<turnstile>\<^sub>d\<^sub>b es : ts \<Longrightarrow> 
-  \<Gamma>\<^sub>1 @ \<Gamma>' @ \<Gamma>\<^sub>2 \<turnstile>\<^sub>d\<^sub>b map_with_idx (\<lambda>k. multiincr (length \<Gamma>') (k + length \<Gamma>\<^sub>1)) es : ts"
+  \<Gamma>\<^sub>1 @ \<Gamma>' @ \<Gamma>\<^sub>2 \<turnstile>\<^sub>d\<^sub>b map_with_idx (length \<Gamma>\<^sub>1) (multiincr (length \<Gamma>')) es : ts"
 proof (induction \<Gamma>')
   case Nil
-  then show ?case by simp
+  thus ?case by simp
 next
   case (Cons t \<Gamma>')
-  hence "\<Gamma>\<^sub>1 @ t # \<Gamma>' @ \<Gamma>\<^sub>2 \<turnstile>\<^sub>d\<^sub>b map_with_idx (\<lambda>k. multiincr (Suc (length \<Gamma>')) (k + length \<Gamma>\<^sub>1)) es : 
-    ts" by simp
-  hence "\<Gamma>\<^sub>1 @ (t # \<Gamma>') @ \<Gamma>\<^sub>2 \<turnstile>\<^sub>d\<^sub>b map_with_idx (\<lambda>k. multiincr (length (t # \<Gamma>')) (k + length \<Gamma>\<^sub>1)) es : 
-    ts" by (simp del: multiincr.simps)
-  thus ?case by blast
+  hence "\<Gamma>\<^sub>1 @ t # \<Gamma>' @ \<Gamma>\<^sub>2 \<turnstile>\<^sub>d\<^sub>b map_with_idx (length \<Gamma>\<^sub>1) (\<lambda>k. multiincr (Suc (length \<Gamma>')) k) es : ts" 
+    by simp
+  hence "\<Gamma>\<^sub>1 @ t # \<Gamma>' @ \<Gamma>\<^sub>2 \<turnstile>\<^sub>d\<^sub>b map_with_idx (length \<Gamma>\<^sub>1) (multiincr (Suc (length \<Gamma>'))) es : ts" 
+    by blast
+  thus ?case by (simp del: multiincr.simps)
 qed
 
 lemma typing_binding_multiincr: "\<Gamma> \<turnstile>\<^sub>d\<^sub>b es : ts \<Longrightarrow> 
-  \<Gamma>' @ \<Gamma> \<turnstile>\<^sub>d\<^sub>b map_with_idx (multiincr (length \<Gamma>')) es : ts"
+  \<Gamma>' @ \<Gamma> \<turnstile>\<^sub>d\<^sub>b map_with_idx 0 (multiincr (length \<Gamma>')) es : ts"
 proof -
   assume "\<Gamma> \<turnstile>\<^sub>d\<^sub>b es : ts"
-  hence "[] @ \<Gamma>' @ \<Gamma> \<turnstile>\<^sub>d\<^sub>b map_with_idx (\<lambda>k. multiincr (length \<Gamma>') (k + length [])) es : ts" 
+  hence "[] @ \<Gamma>' @ \<Gamma> \<turnstile>\<^sub>d\<^sub>b map_with_idx (length []) (multiincr (length \<Gamma>')) es : ts" 
     by (metis typing_binding_multiincr' append_Nil list.size(3))
   thus ?thesis by simp
 qed
@@ -343,7 +364,7 @@ proof (induction \<Gamma> e t rule: typing\<^sub>d.induct)
   with T1 have "\<Gamma> \<turnstile>\<^sub>d\<^sub>b ?es\<^sub>1 @ [?e\<^sub>1'] : [Arrow t\<^sub>1 t\<^sub>2] @ ts\<^sub>1" 
     by (metis typing_bindings_append tc\<^sub>d_bind_cons append_Nil)
   with T1 have TS1: "\<Gamma> \<turnstile>\<^sub>d\<^sub>b ?es\<^sub>1' : ?ts\<^sub>1" by simp
-  with T2 have TS2: "?ts\<^sub>1 @ \<Gamma> \<turnstile>\<^sub>d\<^sub>b map_with_idx (multiincr (length ?es\<^sub>1')) ?es\<^sub>2 : ts\<^sub>2" 
+  with T2 have TS2: "?ts\<^sub>1 @ \<Gamma> \<turnstile>\<^sub>d\<^sub>b map_with_idx 0 (multiincr (length ?es\<^sub>1')) ?es\<^sub>2 : ts\<^sub>2" 
     by (simp add: typing_binding_multiincr)
   from T1 have "[] @ ?ts\<^sub>1 @ \<Gamma> \<turnstile>\<^sub>d (if is_reducible ?e\<^sub>1' then Var\<^sub>d 0 else ?e\<^sub>1') : Arrow t\<^sub>1 t\<^sub>2" by simp
   hence "[] @ ts\<^sub>2 @ ?ts\<^sub>1 @ \<Gamma> \<turnstile>\<^sub>d 
@@ -374,21 +395,7 @@ lemma reapply_let_val [simp]: "value\<^sub>d (reapply_lets es e) = (es = [] \<an
 lemma float_lets_val [simp]: "value\<^sub>d (float_lets e) = value\<^sub>d e"
   by (induction e) (auto simp add: Let_def split: prod.splits)
 
-lemma strip_lets_subst [simp]: "value\<^sub>d v \<Longrightarrow>
-    strip_lets (subst\<^sub>d x v e) = map_with_idx (\<lambda>k. subst\<^sub>d (k + x) (multiincr k 0 v)) (strip_lets e)"
-  by (induction e arbitrary: x v) (auto split: prod.splits)
-
-lemma inner_expr_subst [simp]: "value\<^sub>d v \<Longrightarrow> inner_expr (subst\<^sub>d x v e) = 
-    subst\<^sub>d (length (strip_lets e) + x) (multiincr (length (strip_lets e)) 0 v) (inner_expr e)"
-  by (induction e arbitrary: x v) (auto split: prod.splits)
-
-lemma reapply_let_subst [simp]: "subst\<^sub>d x v (reapply_lets es e) = 
-  reapply_lets (map_with_idx (\<lambda>k. subst\<^sub>d (k + x) (multiincr k 0 v)) es) 
-    (subst\<^sub>d (x + length es) (multiincr (length es) 0 v) e)"
-  by (induction es arbitrary: x v) (simp_all add: reapply_lets_def)
-
-lemma strip_lets_incr [simp]: "strip_lets (incr\<^sub>d x e) = 
-    map_with_idx (\<lambda>k. incr\<^sub>d (k + x)) (strip_lets e)"
+lemma strip_lets_incr [simp]: "strip_lets (incr\<^sub>d x e) = map_with_idx x incr\<^sub>d (strip_lets e)"
   by (induction e arbitrary: x) (auto simp add: comp_def split: prod.splits)
 
 lemma inner_expr_incr [simp]: "inner_expr (incr\<^sub>d x e) = 
@@ -396,103 +403,105 @@ lemma inner_expr_incr [simp]: "inner_expr (incr\<^sub>d x e) =
   by (induction e arbitrary: x) (auto simp add: comp_def split: prod.splits)
 
 lemma reapply_let_incr [simp]: "incr\<^sub>d x (reapply_lets es e) = 
-    reapply_lets (map_with_idx (\<lambda>k. incr\<^sub>d (k + x)) es) (incr\<^sub>d (x + length es) e)"
+    reapply_lets (map_with_idx x incr\<^sub>d es) (incr\<^sub>d (x + length es) e)"
   by (induction es arbitrary: x) (simp_all add: comp_def reapply_lets_def)
 
-lemma float_lets_lemma [simp]: "map_with_idx (multiincr y) (map_with_idx (\<lambda>k. incr\<^sub>d (k + x)) es) = 
-  map_with_idx (\<lambda>k. incr\<^sub>d (k + (x + y))) (map_with_idx (multiincr y) es)"
-proof (induction y)
-  case (Suc y)
-  have "\<And>k. incr\<^sub>d k \<circ> incr\<^sub>d (k + (x + y)) = incr\<^sub>d (Suc (k + (x + y))) \<circ> incr\<^sub>d k" by auto
-  hence "map_with_idx (\<lambda>k. incr\<^sub>d k \<circ> incr\<^sub>d (k + (x + y)) \<circ> multiincr y k) es =
-    map_with_idx (\<lambda>k. incr\<^sub>d (Suc (k + (x + y))) \<circ> incr\<^sub>d k \<circ> multiincr y k) es" by simp
-  with Suc have "map_with_idx (\<lambda>k. incr\<^sub>d k \<circ> multiincr y k) (map_with_idx (\<lambda>k. incr\<^sub>d (k + x)) es) =
-    map_with_idx (\<lambda>k. incr\<^sub>d (k + (x + Suc y))) (map_with_idx (\<lambda>k. incr\<^sub>d k \<circ> multiincr y k) es)" 
-      by simp
-  then show ?case by (simp add: comp_def)
-qed simp_all
+lemma float_lets_lemma [simp]: "z \<le> x \<Longrightarrow> 
+  map_with_idx z (multiincr y) (map_with_idx x incr\<^sub>d es) =
+    map_with_idx (x + y) incr\<^sub>d (map_with_idx z (multiincr y) es)"
+  by (induction es arbitrary: z x) simp_all
 
-lemma float_lets_lemma2 [simp]: "multiincr y 0 (incr\<^sub>d (z + x) e) = 
-    incr\<^sub>d (x + z + y) (multiincr y 0 e)"
-  by (induction y) (simp_all add: add.commute)
-
-lemma float_lets_lemma3 [simp]: "multiincr y z (incr\<^sub>d (z + x) e) = 
-    incr\<^sub>d (x + y + z) (multiincr y z e)"
-  by (induction y) (simp_all add: add.commute)
+lemma float_lets_lemma2 [simp]: "map_with_idx z (multiincr y) 
+  (map_with_idx z (\<lambda>k. subst\<^sub>d (k + x) (multiincr k 0 v)) es) = 
+    map_with_idx z (\<lambda>k. subst\<^sub>d (k + (x + y)) (multiincr k 0 (multiincr y 0 v))) 
+      (map_with_idx z (multiincr y) es)"
+  by (induction es arbitrary: z) (simp_all add: add.commute add.left_commute)
 
 lemma float_lets_incr [simp]: "float_lets (incr\<^sub>d x e) = incr\<^sub>d x (float_lets e)"
 proof (induction e arbitrary: x)
   case (App\<^sub>d e1 e2)
-  thus ?case by (simp add: Let_def incr_above)
+  thus ?case by (simp add: Let_def incr_above add.commute add.left_commute)
 qed (simp_all add: Let_def add.commute)
+
+lemma strip_lets_subst [simp]: "value\<^sub>d v \<Longrightarrow>
+    strip_lets (subst\<^sub>d x v e) = map_with_idx 0 (\<lambda>k. subst\<^sub>d (k + x) (multiincr k 0 v)) (strip_lets e)"
+  by (induction e arbitrary: x v) (auto split: prod.splits)
+
+lemma inner_expr_subst [simp]: "value\<^sub>d v \<Longrightarrow> inner_expr (subst\<^sub>d x v e) = 
+    subst\<^sub>d (length (strip_lets e) + x) (multiincr (length (strip_lets e)) 0 v) (inner_expr e)"
+  by (induction e arbitrary: x v) (auto split: prod.splits)
+
+lemma reapply_let_subst [simp]: "subst\<^sub>d x v (reapply_lets es e) = 
+  reapply_lets (map_with_idx 0 (\<lambda>k. subst\<^sub>d (k + x) (multiincr k 0 v)) es) 
+    (subst\<^sub>d (x + length es) (multiincr (length es) 0 v) e)"
+  by (induction es arbitrary: x v) (simp_all add: reapply_lets_def)
 
 lemma float_lets_subst [simp]: "value\<^sub>d v \<Longrightarrow> 
   float_lets (subst\<^sub>d x v e) = subst\<^sub>d x (float_lets v) (float_lets e)"
 proof (induction e arbitrary: x v)
   case (App\<^sub>d e1 e2)
-  from App\<^sub>d have "value\<^sub>d xv \<Longrightarrow> float_lets (subst\<^sub>d xx xv e1) = subst\<^sub>d xx (float_lets xv) (float_lets e1)" by simp
-  from App\<^sub>d have "value\<^sub>d xv \<Longrightarrow> float_lets (subst\<^sub>d xx xv e2) = subst\<^sub>d xx (float_lets xv) (float_lets e2)" by simp
-  from App\<^sub>d have "value\<^sub>d v" by simp
-
-
   let ?es\<^sub>1 = "strip_lets (float_lets e1)"
-  let ?es\<^sub>1\<^sub>s = "map_with_idx (\<lambda>k. subst\<^sub>d (k + x) (multiincr k 0 (float_lets v))) ?es\<^sub>1"
-  let ?e\<^sub>1' = "inner_expr (float_lets e1)"
-  let ?e\<^sub>1\<^sub>s' = "subst\<^sub>d (length ?es\<^sub>1 + x) (multiincr (length ?es\<^sub>1) 0 (float_lets v)) ?e\<^sub>1'"
   let ?es\<^sub>2 = "strip_lets (float_lets e2)"
-  let ?es\<^sub>2\<^sub>s = "map_with_idx (\<lambda>k. subst\<^sub>d (k + x) (multiincr k 0 (float_lets v))) ?es\<^sub>2"
-  let ?es\<^sub>1' = "if is_reducible ?e\<^sub>1' then ?es\<^sub>1 @ [?e\<^sub>1'] else ?es\<^sub>1"
-  let ?es\<^sub>1\<^sub>s' = "if is_reducible ?e\<^sub>1\<^sub>s' then ?es\<^sub>1\<^sub>s @ [?e\<^sub>1\<^sub>s'] else ?es\<^sub>1\<^sub>s"
-
-  from App\<^sub>d have X: "(map_with_idx (\<lambda>k. subst\<^sub>d (k + (x + length ?es\<^sub>1')) (multiincr k 0 (multiincr (length ?es\<^sub>1') 0 (float_lets v)))) 
-      (map_with_idx (multiincr (length ?es\<^sub>1')) ?es\<^sub>2)) = (map_with_idx (multiincr (length ?es\<^sub>1\<^sub>s')) ?es\<^sub>2\<^sub>s)"
-    by simp
-
-  have Y: "subst\<^sub>d (x + length ?es\<^sub>1' + length (map_with_idx (multiincr (length ?es\<^sub>1')) ?es\<^sub>2)) 
-    (multiincr (length (map_with_idx (multiincr (length ?es\<^sub>1')) ?es\<^sub>2)) 0 (multiincr (length ?es\<^sub>1') 0 (float_lets v))) 
-      (multiincr (length ?es\<^sub>2) 0 (if is_reducible ?e\<^sub>1' then Var\<^sub>d 0 else ?e\<^sub>1')) =
-        multiincr (length ?es\<^sub>2\<^sub>s) 0 (if is_reducible ?e\<^sub>1\<^sub>s' then Var\<^sub>d 0 else ?e\<^sub>1\<^sub>s')" by simp
-
-
-  have "multiincr (length ?es\<^sub>1\<^sub>s') (length ?es\<^sub>2\<^sub>s) (subst\<^sub>d (length ?es\<^sub>2 + x) 
-    (multiincr (length ?es\<^sub>2) 0 (float_lets v)) (inner_expr (float_lets e2))) =
-      subst\<^sub>d (x + length ?es\<^sub>1' + length (map_with_idx (multiincr (length ?es\<^sub>1')) ?es\<^sub>2)) 
-        (multiincr (length (map_with_idx (multiincr (length ?es\<^sub>1')) ?es\<^sub>2)) 0 
-            (multiincr (length ?es\<^sub>1') 0 (float_lets v))) (multiincr (length ?es\<^sub>1') (length ?es\<^sub>2) 
-            (inner_expr (float_lets e2)))" by simp
-  with App\<^sub>d X Y show ?case by (simp add: Let_def)
+  have A: "length ?es\<^sub>2 + (length ?es\<^sub>1 + x) = x + length ?es\<^sub>1 + length ?es\<^sub>2" by simp
+  have B: "length ?es\<^sub>1 + (length ?es\<^sub>2 + x) = x + length ?es\<^sub>1 + length ?es\<^sub>2" by simp
+  from App\<^sub>d show ?case by (simp add: Let_def A B)
 qed (simp_all add: Let_def add.commute)
 
-theorem correctness\<^sub>f\<^sub>l [simp]: "e \<leadsto>\<^sub>d e' \<Longrightarrow> iter (\<leadsto>\<^sub>d) (float_lets e) (float_lets e')"
+primrec strip_lets_eval_prop :: "expr\<^sub>d \<Rightarrow> expr\<^sub>d list \<Rightarrow> expr\<^sub>d \<Rightarrow> bool" where
+  "strip_lets_eval_prop e' [] e = (e \<leadsto>\<^sub>d e')"
+| "strip_lets_eval_prop e' (ee # es) e = 
+    ((\<exists>ee'. ee \<leadsto>\<^sub>d ee' \<and> e' =  Let\<^sub>d ee' (reapply_lets es e)) \<or> 
+      (value\<^sub>d ee \<and> e' = subst\<^sub>d 0 ee (reapply_lets es e)))"
+
+lemma eval_strip_lets [simp]: "e \<leadsto>\<^sub>d e' \<Longrightarrow> strip_lets_eval_prop e' (strip_lets e) (inner_expr e)"
+  by (induction e e' rule: eval\<^sub>d.induct) simp_all
+
+theorem correctness\<^sub>f\<^sub>l [simp]: "e \<leadsto>\<^sub>d e' \<Longrightarrow> 
+  \<exists>e''. float_lets e \<leadsto>\<^sub>d e'' \<and> float_lets e'' = float_lets e'"
 proof (induction e e' rule: eval\<^sub>d.induct)
   case (ev\<^sub>d_app1 e\<^sub>1 e\<^sub>1' e\<^sub>2)
-  thus ?case by simpx 
+  then obtain e\<^sub>1'' where "float_lets e\<^sub>1 \<leadsto>\<^sub>d e\<^sub>1'' \<and> float_lets e\<^sub>1'' = float_lets e\<^sub>1'" by blast
+
+
+  have "(let es\<^sub>1 = strip_lets (float_lets e\<^sub>1); e\<^sub>1' = inner_expr (float_lets e\<^sub>1);
+         es\<^sub>2 = strip_lets (float_lets e\<^sub>2); es\<^sub>1' = if is_reducible e\<^sub>1' then es\<^sub>1 @ [e\<^sub>1'] else es\<^sub>1
+     in reapply_lets es\<^sub>1'
+         (reapply_lets (map_with_idx 0 (multiincr (length es\<^sub>1')) es\<^sub>2)
+           (App\<^sub>d (multiincr (length es\<^sub>2) 0 (if is_reducible e\<^sub>1' then Var\<^sub>d 0 else e\<^sub>1'))
+             (multiincr (length es\<^sub>1') (length es\<^sub>2) (inner_expr (float_lets e\<^sub>2)))))) \<leadsto>\<^sub>d
+    e'' \<and>
+    float_lets e'' =
+    (let es\<^sub>1 = strip_lets (float_lets e\<^sub>1'); e\<^sub>1' = inner_expr (float_lets e\<^sub>1');
+         es\<^sub>2 = strip_lets (float_lets e\<^sub>2); es\<^sub>1' = if is_reducible e\<^sub>1' then es\<^sub>1 @ [e\<^sub>1'] else es\<^sub>1
+     in reapply_lets es\<^sub>1'
+         (reapply_lets (map_with_idx 0 (multiincr (length es\<^sub>1')) es\<^sub>2)
+           (App\<^sub>d (multiincr (length es\<^sub>2) 0 (if is_reducible e\<^sub>1' then Var\<^sub>d 0 else e\<^sub>1'))
+             (multiincr (length es\<^sub>1') (length es\<^sub>2) (inner_expr (float_lets e\<^sub>2))))))" by simp
+  hence "float_lets (App\<^sub>d e\<^sub>1 e\<^sub>2) \<leadsto>\<^sub>d e'' \<and> float_lets e'' = float_lets (App\<^sub>d e\<^sub>1' e\<^sub>2)" by simp
+  thus ?case by blast
 next
   case (ev\<^sub>d_app2 e\<^sub>1 e\<^sub>2 e\<^sub>2')
-  then show ?case by simpx
-next
-  case (ev\<^sub>d_app3 e\<^sub>2 t e\<^sub>1)
   then show ?case by simp
 next
+  case (ev\<^sub>d_app3 e\<^sub>2 t e\<^sub>1)
+  hence "float_lets (App\<^sub>d (Lam\<^sub>d t e\<^sub>1) e\<^sub>2) \<leadsto>\<^sub>d subst\<^sub>d 0 (float_lets e\<^sub>2) (float_lets e\<^sub>1) \<and> 
+    float_lets (subst\<^sub>d 0 (float_lets e\<^sub>2) (float_lets e\<^sub>1)) = float_lets (subst\<^sub>d 0 e\<^sub>2 e\<^sub>1)" by simp
+  thus ?case by blast
+next
   case (ev\<^sub>d_let1 e\<^sub>1 e\<^sub>1' e\<^sub>2)
+  then obtain e\<^sub>1'' where "float_lets e\<^sub>1 \<leadsto>\<^sub>d e\<^sub>1'' \<and> float_lets e\<^sub>1'' = float_lets e\<^sub>1'" by blast
 
-  have "iter (\<leadsto>\<^sub>d)
-     (let es\<^sub>1 = strip_lets (float_lets e\<^sub>1)
-      in reapply_lets es\<^sub>1
-          (Let\<^sub>d (inner_expr (float_lets e\<^sub>1)) (multiincr (length es\<^sub>1) (Suc 0) (float_lets e\<^sub>2))))
-     (let es\<^sub>1 = strip_lets (float_lets e\<^sub>1')
-      in reapply_lets es\<^sub>1
-          (Let\<^sub>d (inner_expr (float_lets e\<^sub>1')) (multiincr (length es\<^sub>1) (Suc 0) (float_lets e\<^sub>2))))" by simp
-  thus ?case by simp
+
+  have "float_lets (Let\<^sub>d e\<^sub>1 e\<^sub>2) \<leadsto>\<^sub>d e'' \<and> float_lets e'' = float_lets (Let\<^sub>d e\<^sub>1' e\<^sub>2)" by simp 
+  thus ?case by blast
 next
   case (ev\<^sub>d_let2 e\<^sub>1 e\<^sub>2)
-  hence "Let\<^sub>d (float_lets e\<^sub>1) (float_lets e\<^sub>2) \<leadsto>\<^sub>d subst\<^sub>d 0 (float_lets e\<^sub>1) (float_lets e\<^sub>2)" by simp
-  hence "iter (\<leadsto>\<^sub>d) (Let\<^sub>d (float_lets e\<^sub>1) (float_lets e\<^sub>2)) (subst\<^sub>d 0 (float_lets e\<^sub>1) (float_lets e\<^sub>2))"
-    by simp
-  with ev\<^sub>d_let2 show ?case by (simp add: Let_def)
+  hence "float_lets (Let\<^sub>d e\<^sub>1 e\<^sub>2) \<leadsto>\<^sub>d subst\<^sub>d 0 (float_lets e\<^sub>1) (float_lets e\<^sub>2) \<and>
+    float_lets (subst\<^sub>d 0 (float_lets e\<^sub>1) (float_lets e\<^sub>2)) = float_lets (subst\<^sub>d 0 e\<^sub>1 e\<^sub>2)" by simp
+  thus ?case by blast
 qed
 
 lemma iter_correct\<^sub>f\<^sub>l [simp]: "iter (\<leadsto>\<^sub>d) e e' \<Longrightarrow> iter (\<leadsto>\<^sub>d) (float_lets e) (float_lets e')"
-  by (induction e e' rule: iter.induct) (simp, metis correctness\<^sub>f\<^sub>l iter_append)
+  by (induction e e' rule: iter.induct) (simp, metisx correctness\<^sub>f\<^sub>l iter_append)
 
 end
